foldctree

theories/Interp/FoldCTree.v
@@ -1,4 +1,5 @@
 (* begin hide *)
+Unset Universe Checking.
 
 From ExtLib Require Import
      Structures.Functor
@@ -34,203 +35,259 @@ Section FoldCTree.
 
     (** Specialization to [M = ctree F (B01 +' D)] *)
     Context {E F C D: Type -> Type} {X : Type}
-      {h : E ~> ctree F (B01 +' D)} {g : bool -> B01 +' C ~> ctree F (B01 +' D)}.
+      {h : E ~> ctree F D} {g : C ~> ctree F D}.
 
     (** ** [interpE] and constructors *)
+    Definition fold_ctree : forall [T], ctree E C T -> ctree F D T :=
+      fold mstuck mstep h g.
+      (* fold (mstuck (M := ctree F D)) (mstep (M := ctree F D)) h (mbr (M := ctree F D)) g. *)
+      (* fold (fun T => Stuck: ctree F D T) (Step (Ret tt)) h g. *)
 
     (** Unfolding of [fold]. *)
-    Notation fold_ h g t :=
+    Notation fold_ctree_ t :=
       (match observe t with
        | RetF r => Ret r
-	     | VisF e k => bind (h _ e) (fun x => Guard (fold h g (k x)))
-	     | BrF b c k => bind (g b _ c) (fun x => Guard (fold h g (k x)))
+       | StuckF => Stuck
+       | GuardF t => Guard (fold_ctree t)
+       | StepF t => Step (Guard (fold_ctree t))
+	     | VisF e k => CTree.bind (h _ e) (fun x => Guard (fold_ctree (k x)))
+	     | BrF c k => CTree.bind (g _ c) (fun x => Guard (fold_ctree (k x)))
        end)%function.
 
     (** Unfold lemma. *)
-    Lemma unfold_fold (t: ctree E (B01 +' C) X):
-      fold h g t ≅ fold_ h g t.
+    Lemma unfold_fold_ctree (t: ctree E C X):
+      fold_ctree t ≅ fold_ctree_ t.
     Proof.
-      unfold fold, Basics.iter, MonadIter_ctree, mbr, MonadBr_ctree, CTree.branch.
+      unfold fold_ctree, fold, Basics.iter, MonadIter_ctree, mbr, MonadBr_ctree, CTree.branch.
       rewrite unfold_iter.
       destruct (observe t); cbn.
+      - now rewrite ?bind_ret_l.
+      - now rewrite ?bind_stuck.
+      - setoid_rewrite bind_step.
+        setoid_rewrite bind_step.
+        setoid_rewrite bind_ret_l.
+        now setoid_rewrite bind_ret_l.
       - now rewrite ?bind_ret_l.
       - now rewrite bind_map, ?bind_ret_l.
       - now rewrite bind_map.
     Qed.
 
-    Lemma fold_ret (x: X):
-      fold h g (Ret x) ≅ Ret x.
-    Proof. now rewrite unfold_fold. Qed.
+    Lemma fold_ctree_ret (x: X):
+      fold_ctree (Ret x) ≅ Ret x.
+    Proof. now rewrite unfold_fold_ctree. Qed.
 
-    Lemma fold_vis {U} (e: E U) (k: U -> ctree E (B01 +' C) X) :
-      fold h g (Vis e k) ≅ x <- h _ e;; Guard (fold h g (k x)).
-    Proof. now rewrite unfold_fold. Qed.
+    Lemma fold_ctree_vis {U} (e: E U) (k: U -> ctree E C X) :
+      fold_ctree (Vis e k) ≅ x <- h _ e;; Guard (fold_ctree (k x)).
+    Proof. now rewrite unfold_fold_ctree. Qed.
 
-    Lemma fold_br {U} b (c : (B01 +' C) U) (k: _ -> ctree E (B01 +' C) X) :
-      fold h g (Br b c k) ≅ x <- g b _ c;; Guard (fold h g (k x)).
-    Proof. now rewrite unfold_fold. Qed.
+    Lemma fold_ctree_stuck :
+      fold_ctree (Stuck : ctree E C X) ≅ Stuck.
+    Proof. now rewrite unfold_fold_ctree. Qed.
 
-    #[global] Instance fold_equ :
-      Proper (equ eq ==> equ eq) (fold h g (T := X)).
+    Lemma fold_ctree_guard (t : ctree E C X) :
+      fold_ctree (Guard t) ≅ Guard (fold_ctree t).
+    Proof. now rewrite unfold_fold_ctree. Qed.
+
+    Lemma fold_ctree_step (t : ctree E C X) :
+      fold_ctree (Step t) ≅ Step (Guard (fold_ctree t)).
+    Proof. now rewrite unfold_fold_ctree. Qed.
+
+    Lemma fold_ctree_br {U} (c : C U) (k: _ -> ctree E C X) :
+      fold_ctree (Br c k) ≅ x <- g _ c;; Guard (fold_ctree (k x)).
+    Proof. now rewrite unfold_fold_ctree. Qed.
+
+    #[global] Instance fold_ctree_equ :
+      Proper (equ eq ==> equ eq) (fold_ctree (T := X)).
     Proof.
       cbn.
-      coinduction ? CIH.
+      coinduction r CIH.
       intros * EQ; step in EQ.
-      rewrite 2 unfold_fold.
+      rewrite 2 unfold_fold_ctree.
       inv EQ; auto.
-      - cbn -[ebt].
-        upto_bind_eq.
-        constructor; intros ?; auto.
-      - cbn -[ebt].
-        upto_bind_eq.
-        constructor; intros ?; auto.
+      - constructor; eauto.
+      - constructor; eauto.
+        cstep; constructor; eauto.
+      - upto_bind_eq.
+        intros ?; constructor; auto.
+      - upto_bind_eq.
+        intros ?; constructor; auto.
     Qed.
 
     (** Unfolding of [interp]. *)
+
     Notation interp_ h t :=
       (match observe t with
        | RetF r => Ret r
+       | StuckF => Stuck
+       | GuardF t => Guard (interp h t)
+       | StepF  t => Step  (Guard (interp h t))
 	     | VisF e k => bind (h _ e) (fun x => Guard (interp h (k x)))
-	     | BrF b c k => bind (mbr b c) (fun x => Guard (interp h (k x)))
+	     | BrF c k => bind (mbr _ c) (fun x => Guard (interp h (k x)))
        end)%function.
 
     (** Unfold lemma. *)
-    Lemma unfold_interp `{C -< D} (t: ctree E (B01 +' C) X):
+    Lemma unfold_interp `{C -< D} (t: ctree E C X):
       interp h t ≅ interp_ h t.
     Proof.
       unfold interp,fold, Basics.iter, MonadIter_ctree, mbr, MonadBr_ctree, CTree.branch.
       rewrite unfold_iter.
       destruct (observe t); cbn.
       - now rewrite ?bind_ret_l.
+      - now rewrite bind_stuck.
+      - repeat setoid_rewrite bind_step.
+        step; constructor.
+        now rewrite ?bind_ret_l.
+      - now rewrite bind_ret_l.
       - now rewrite bind_map, ?bind_ret_l.
       - now rewrite bind_map.
     Qed.
 
     Lemma interp_ret `{C -< D} (x: X):
-      interp h (Ret x : ctree E (B01 +' C) X) ≅ Ret x.
+      interp h (Ret x : ctree E C X) ≅ Ret x.
     Proof. now rewrite unfold_interp. Qed.
 
-    Lemma interp_vis `{C -< D} {U} (e: E U) (k: U -> ctree E (B01 +' C) X) :
+    Lemma interp_vis `{C -< D} {U} (e: E U) (k: U -> ctree E C X) :
       interp h (Vis e k) ≅ x <- h _ e;; Guard (interp h (k x)).
     Proof. now rewrite unfold_interp. Qed.
 
-    Lemma interp_br `{C -< D} {U} b (c : (B01 +' C) U) (k: _ -> ctree E (B01 +' C) X) :
-      interp h (Br b c k) ≅ x <- branch b c;; Guard (interp h (k x)).
+    Lemma interp_guard `{C -< D} (t : ctree E C X) :
+      interp h (Guard t) ≅ Guard (interp h t).
+    Proof. now rewrite unfold_interp. Qed.
+
+    Lemma interp_step `{C -< D} (t : ctree E C X) :
+      interp h (Step t) ≅ Step (Guard (interp h t)).
+    Proof. now rewrite unfold_interp. Qed.
+
+    Lemma interp_br `{C -< D} {U} (c : C U) (k: _ -> ctree E C X) :
+      interp h (Br c k) ≅ x <- branch c;; Guard (interp h (k x)).
     Proof. now rewrite unfold_interp. Qed.
 
     #[global] Instance interp_equ `{C -< D} {R} :
-      Proper (equ R ==> equ R) (interp (B := C) (M := ctree F (B01 +' D)) h (T := X)).
+      Proper (equ R ==> equ R) (interp (B := C) (M := ctree F D) h (T := X)).
     Proof.
       cbn.
-      coinduction ? CIH.
+      coinduction r CIH.
       intros * EQ; step in EQ.
       rewrite 2 unfold_interp.
       inv EQ.
       - constructor; auto.
-      - cbn -[ebt].
-        upto_bind_eq.
-        constructor; intros ?; auto.
-      - cbn -[ebt].
-        upto_bind_eq.
-        constructor; intros ?; auto.
+      - constructor; auto.
+      - constructor; auto.
+      - constructor; cstep; constructor; auto.
+      - upto_bind_eq; intros.
+        constructor; eauto.
+      - upto_bind_eq; intros.
+        constructor; eauto.
     Qed.
 
     (** Unfolding of [refine]. *)
     Notation refine_ g t :=
       (match observe t with
        | RetF r => Ret r
-	     | VisF e k => bind (mtrigger e) (fun x => Guard (refine g (k x)))
-	     | BrF b c k => bind (g b _ c) (fun x => Guard (refine g (k x)))
+       | StuckF => Stuck
+       | GuardF t => Guard (refine g t)
+       | StepF  t => Step  (Guard (refine g t))
+		   | VisF e k => bind (mtrigger e) (fun x => Guard (refine g (k x)))
+	     | BrF c k => bind (g _ c) (fun x => Guard (refine g (k x)))
        end)%function.
 
     (** Unfold lemma. *)
-    Lemma unfold_refine `{E -< F} (t: ctree E (B01 +' C) X):
+    Lemma unfold_refine `{E -< F} (t: ctree E C X):
       refine g t ≅ refine_ g t.
     Proof.
       unfold refine,fold, Basics.iter, MonadIter_ctree, mbr, MonadBr_ctree, CTree.branch.
       rewrite unfold_iter.
       destruct (observe t); cbn.
       - now rewrite ?bind_ret_l.
+      - now rewrite bind_stuck.
+      - repeat setoid_rewrite bind_step.
+        step; constructor.
+        now rewrite ?bind_ret_l.
+      - now rewrite bind_ret_l.
       - now rewrite bind_map, ?bind_ret_l.
       - now rewrite bind_map.
     Qed.
 
     Lemma refine_ret `{E -< F} (x: X):
-      refine g (Ret x : ctree E (B01 +' C) X) ≅ Ret x.
+      refine g (Ret x : ctree E C X) ≅ Ret x.
     Proof. now rewrite unfold_refine. Qed.
 
-    Lemma refine_vis `{E -< F} {U} (e: E U) (k: U -> ctree E (B01 +' C) X) :
+    Lemma refine_vis `{E -< F} {U} (e: E U) (k: U -> ctree E C X) :
       refine g (Vis e k) ≅ x <- trigger e;; Guard (refine g (k x)).
     Proof. now rewrite unfold_refine. Qed.
 
-    Lemma refine_br `{E -< F} {U} b (c : (B01 +' C) U) (k: _ -> ctree E (B01 +' C) X) :
-      refine g (Br b c k) ≅ x <- g b _ c;; Guard (refine g (k x)).
+    Lemma refine_guard `{E -< F} (t: ctree E C X) :
+      refine g (Guard t) ≅ Guard (refine g t).
+    Proof. now rewrite unfold_refine. Qed.
+
+    Lemma refine_step `{E -< F} (t: ctree E C X) :
+      refine g (Step t) ≅ Step (Guard (refine g t)).
+    Proof. now rewrite unfold_refine. Qed.
+
+    Lemma refine_br `{E -< F} {U} (c : C U) (k: _ -> ctree E C X) :
+      refine g (Br c k) ≅ x <- g _ c;; Guard (refine g (k x)).
     Proof. now rewrite unfold_refine. Qed.
 
     #[global] Instance refine_equ `{E -< F} :
       Proper (equ eq ==> equ eq) (refine (E := E) (M := ctree F _) g (T := X)).
     Proof.
       cbn.
-      coinduction ? CIH.
+      coinduction r CIH.
       intros * EQ; step in EQ.
       rewrite 2 unfold_refine.
-      inv EQ; auto.
-      - cbn -[ebt].
-        upto_bind_eq.
-        constructor; intros ?; auto.
-      - cbn -[ebt].
-        upto_bind_eq.
-        constructor; intros ?; auto.
+      inv EQ; try constructor; auto.
+      - cstep; constructor; auto.
+      - upto_bind_eq.
+        intros ?; constructor; auto.
+      - upto_bind_eq.
+        intros ?; constructor; auto.
     Qed.
 
   End With_Params.
 
-  (** The following fact specialises further [interp] so that events are implemented into ctrees whose index for branches is unchanged.
-      Most likely, this is the case in all applications.
-   *)
-  Lemma interp_guard {E F C X} `{B1 -< C} (h' : E ~> ctree F (B01 +' C)) (t: ctree E (B01 +' C) X):
-    interp h' (Guard t) ≅ Guard (Guard (interp h' t)).
-  Proof.
-    rewrite unfold_interp. setoid_rewrite bind_br.
-    apply equ_BrF. intro.
-    rewrite bind_ret_l. reflexivity.
-  Qed.
+  Arguments fold_ctree {E F C D} h g [T].
 
   Section FoldBind.
 
     Context {E F C D: Type -> Type} {X : Type}.
 
-    Lemma fold_bind (h : E ~> ctree F (B01 +' D)) (g : bool -> (B01 +' C) ~> ctree F (B01 +' D)) {S} (t : ctree E (B01 +' C) X) (k : X -> ctree _ _ S) :
-      fold h g (t >>= k) ≅ fold h g t >>= (fun x => fold h g (k x)).
+    Lemma fold_ctree_bind (h : E ~> ctree F D) (g : C ~> ctree F D) {S} (t : ctree E C X) (k : X -> ctree _ _ S) :
+      fold_ctree h g (t >>= k) ≅ fold_ctree h g t >>= (fun x => fold_ctree h g (k x)).
     Proof.
       revert t.
-      coinduction X' CIH.
+      coinduction r CIH.
       intros t.
-      rewrite unfold_bind, (unfold_fold t).
-      desobs t; cbn -[ebt].
+      rewrite unfold_bind, (unfold_fold_ctree t).
+      desobs t.
       - now rewrite bind_ret_l.
-      - rewrite fold_vis, bind_bind.
-        upto_bind_eq.
+      - now rewrite bind_stuck, fold_ctree_stuck.
+      - rewrite bind_step, fold_ctree_step, bind_guard.
+        constructor; cstep; constructor.
+        auto.
+      - rewrite bind_guard, fold_ctree_guard.
+        constructor; auto.
+      - rewrite fold_ctree_vis, bind_bind.
+        upto_bind_eq; intros.
         rewrite bind_guard.
         now constructor.
-      - rewrite fold_br, bind_bind.
-        upto_bind_eq.
+      - rewrite fold_ctree_br, bind_bind.
+        upto_bind_eq; intros.
         rewrite bind_guard.
         now constructor.
     Qed.
 
-    Lemma interp_bind (h : E ~> ctree F (B01 +' D)) `{C -< D} {S} (t : ctree E (B01 +' C) X) (k : X -> ctree _ _ S) :
+    Lemma interp_bind (h : E ~> ctree F D) `{C -< D} {S} (t : ctree E C X) (k : X -> ctree _ _ S) :
       interp h (t >>= k) ≅ interp h t >>= (fun x => interp h (k x)).
     Proof.
       unfold interp.
-      now rewrite fold_bind.
+      now setoid_rewrite fold_ctree_bind.
     Qed.
 
-    Lemma refine_bind (g : bool -> (B01 +' C) ~> ctree F (B01 +' D)) `{E -< F} {S} (t : ctree E (B01 +' C) X) (k : X -> ctree _ _ S) :
+    Lemma refine_bind (g : C ~> ctree F D) `{E -< F} {S} (t : ctree E C X) (k : X -> ctree _ _ S) :
       refine g (t >>= k) ≅ refine g t >>= (fun x => refine g (k x)).
     Proof.
       unfold refine.
-      now rewrite fold_bind.
+      now setoid_rewrite fold_ctree_bind.
     Qed.
 
   End FoldBind.
@@ -246,21 +303,21 @@ Module CounterExample.
   Inductive VoidE : Type -> Type :=
   | voidE : VoidE void.
 
-  Notation B012 := (B01 +' B2).
-  #[local] Definition t1 := Ret 1 : ctree VoidE B012 nat.
-  #[local] Definition t2 := brD2 (Ret 1) (x <- trigger voidE;; match x : void with end) : ctree VoidE B012 nat.
+  (* Notation B012 := (B01 +' B2). *)
+  #[local] Definition t1 := Ret 1 : ctree VoidE B2 nat.
+  #[local] Definition t2 := br2 (Ret 1) (x <- trigger voidE;; match x : void with end) : ctree VoidE B2 nat.
 
   Goal t1 ~ t2.
   Proof.
     unfold t1, t2.
-    rewrite brD2_commut.
-    rewrite brD2_is_stuck. reflexivity.
+    rewrite br2_commut.
+    rewrite br2_is_stuck. reflexivity.
     red. intros. intro. inv_trans.  destruct x.
   Qed.
 
-  #[local] Definition h : VoidE ~> ctree VoidE B012.
+  #[local] Definition h : VoidE ~> ctree VoidE B2.
   Proof.
-    intros. destruct H. exact (Step stuckD).
+    intros. destruct X. exact (Step Stuck).
   Defined.
 
   Example interpE_sbsisim_counterexample : ~ (interp h t1 ~ interp h t2).
@@ -268,7 +325,7 @@ Module CounterExample.
     red. intros. unfold t2 in H.
     playR in H.
     rewrite unfold_interp. cbn. setoid_rewrite bind_br.
-    eapply trans_brD with (x := false).
+    eapply trans_br with (x := false).
     2: { rewrite bind_ret_l. reflexivity. }
     apply trans_guard. setoid_rewrite unfold_interp. cbn. rewrite bind_step. etrans.
     rewrite unfold_interp in TR. unfold t1, h in TR. cbn in TR. inv_trans.
@@ -278,7 +335,7 @@ End CounterExample.
 
 Section epsilon_interp_theory.
 
-  Lemma interp_productive {E C F X} (h : E ~> ctree F (B01 +' C)) : forall (t : ctree E (B01 +' C) X),
+  Lemma interp_productive {E C F X} (h : E ~> ctree F C) : forall (t : ctree E C X),
       productive (interp h t) -> productive t.
   Proof.
     intros. inversion H;
@@ -292,7 +349,7 @@ Section epsilon_interp_theory.
   Qed.
 
   Lemma epsilon_interp : forall {E C F X}
-                          (h : E ~> ctree F (B01 +' C)) (t t' : ctree E (B01 +' C) X),
+                           (h : E ~> ctree F C) (t t' : ctree E C X),
       epsilon t t' -> epsilon (interp h t) (interp h t').
   Proof.
     intros. red in H. setoid_rewrite (ctree_eta t). setoid_rewrite (ctree_eta t').
@@ -300,34 +357,35 @@ Section epsilon_interp_theory.
     induction H.
     - constructor. rewrite H. reflexivity.
     - rewrite unfold_interp. cbn. setoid_rewrite bind_br.
-      apply EpsilonBr with (x := x). rewrite bind_ret_l.
-      simpl. eapply EpsilonBr with (x:=tt). apply IHepsilon_.
+      apply epsilon_br with (x := x). rewrite bind_ret_l.
+      simpl. eapply epsilon_guard. apply IHepsilon_.
+    - rewrite unfold_interp. cbn.
+      now apply epsilon_guard.
   Qed.
 
 End epsilon_interp_theory.
 
-Lemma interp_ret_inv {E F B X} (h : E ~> ctree F (B01 +' B)) :
-  forall (t : ctree E (B01 +' B) X) r,
+Lemma interp_ret_inv {E F B X} (h : E ~> ctree F B) :
+  forall (t : ctree E B X) r,
   interp h t ≅ Ret r -> t ≅ Ret r.
 Proof.
   intros. setoid_rewrite (ctree_eta t) in H. setoid_rewrite (ctree_eta t).
-  destruct (observe t) eqn:?.
+  destruct (observe t) eqn:?; try now inv_equ.
   - rewrite interp_ret in H. step in H. inv H. reflexivity.
   - rewrite interp_vis in H. apply ret_equ_bind in H as (? & ? & ?). step in H0. inv H0.
-  - rewrite interp_br in H. setoid_rewrite bind_br in H. step in H. inv H.
 Qed.
 
-Lemma bind_guard_r {E B X Y} : forall (t : ctree E (B01 +' B) X) (k : X -> ctree E (B01 +' B) Y),
-  x <- t;; Guard (k x) ≅ x <- (x <- t;; Guard (Ret x));; k x.
+Lemma bind_guard_r {E B X Y} : forall (t : ctree E B X) (k : X -> ctree E B Y),
+    x <- t;; Guard (k x) ≅ x <- (x <- t;; Guard (Ret x));; k x.
 Proof.
-  intros. rewrite bind_bind. upto_bind_eq. rewrite bind_guard. setoid_rewrite bind_ret_l. reflexivity.
+  intros. rewrite bind_bind. upto_bind_eq; intros ?. rewrite bind_guard. setoid_rewrite bind_ret_l. reflexivity.
 Qed.
 
 Lemma trans_val_interp {E F B X}
-  (h : E ~> ctree F (B01 +' B)) :
-  forall (t u : ctree E (B01 +' B) X) (v : X),
+  (h : E ~> ctree F B) :
+  forall (t u : ctree E B X) (v : X),
   trans (val v) t u ->
-  trans (val v) (interp h t) stuckD.
+  trans (val v) (interp h t) Stuck.
 Proof.
   intros.
   apply trans_val_epsilon in H as []. subs.
@@ -337,22 +395,22 @@ Proof.
 Qed.
 
 Lemma trans_tau_interp {E F B X}
-  (h : E ~> ctree F (B01 +' B)) :
-  forall (t u : ctree E (B01 +' B) X),
-  trans tau t u ->
-  trans tau (interp h t) (Guard (interp h u)).
+  (h : E ~> ctree F B) :
+  forall (t u : ctree E B X),
+  trans τ t u ->
+  trans τ (interp h t) (Guard (interp h u)).
 Proof.
   intros.
-  apply trans_tau_epsilon in H as (? & ? & ? & ? & ? & ?). subs.
+  apply trans_τ_epsilon in H as (? & ? & ?). subs.
   eapply epsilon_interp in H.
   eapply epsilon_trans; [apply H |].
-  rewrite interp_br, bind_branch.
-  apply (trans_brS _ (fun x3 : x => Guard (interp h (x1 x3)))).
+  rewrite interp_step.
+  etrans.
 Qed.
 
 Lemma trans_obs_interp_step {E F B X Y}
-  (h : E ~> ctree F (B01 +' B)) :
-  forall (t u : ctree E (B01 +' B) X) u' (e : E Y) x l,
+  (h : E ~> ctree F B) :
+  forall (t u : ctree E B X) u' (e : E Y) x l,
   trans (obs e x) t u ->
   trans l (h _ e) u' ->
   ~ is_val l ->
@@ -371,10 +429,10 @@ Proof.
 Qed.
 
 Lemma trans_obs_interp_pure {E F B X Y}
-  (h : E ~> ctree F (B01 +' B)) :
-  forall (t u : ctree E (B01 +' B) X) (e : E Y) x,
+  (h : E ~> ctree F B) :
+  forall (t u : ctree E B X) (e : E Y) x,
   trans (obs e x) t u ->
-  trans (val x) (h _ e) stuckD ->
+  trans (val x) (h _ e) Stuck ->
   epsilon (interp h t) (Guard (interp h u)).
 Proof.
   intros t u e x TR TRh.
